Prove soundness of apply_idx_related_transfs

fiat2/src/fiat2/IndexTransf2.v
@@ -20,6 +20,12 @@ Proof.
   repeat case_match; cbn; congruence.
 Qed.
 
+Ltac NoDup_map_record_sort :=
+  eapply Permutation_NoDup;
+  [ eapply Permutation_map, Permuted_record_sort
+  | cbn; repeat constructor; intuition idtac;
+    destruct_In; auto ].
+
 Section compo_idx.
   Context {tenv : map.map string type} {tenv_ok : map.ok tenv}.
   Context {width: Z} {word: word.word width} {word_ok: word.ok word}.
@@ -171,7 +177,9 @@ Section WithMap.
       Context {idx : IndexInterface2.index} {idx_wf : value -> value -> Prop} {idx_ok : ok idx idx_wf}.
       Context (id_tag aux_tag: string).
       Context (H_tags_diff : id_tag <> aux_tag).
-      Context (tbl : string).
+
+      Section WithGlobal.
+        Context (tbl : string).
 
       Definition create_aux_write_head (free_vars : list string) (c : command) :=
         match c with
@@ -193,24 +201,10 @@ Section WithMap.
       Definition transf_to_idx' (free_vars : list string) (c : command) : command :=
         fold_command_with_global tbl create_aux_write_head create_aux_read_head free_vars c.
 
-      Definition transf_to_idx (free_vars : list string) (c : command) : command :=
-        match c with
-        | CLetMut e tbl c =>
-            CLetMut (ERecord [(id_tag, e); (aux_tag, substitute ((hole, e) :: nil) free_vars to_idx)]) tbl
-              (transf_to_idx' free_vars c)
-        | _ => c
-        end.
-
-      Definition transf_to_idx_ty (tbl_ty : type) :=
+      Definition aux_ty (tbl_ty : type) :=
         TRecord
           (record_sort
              [(id_tag, tbl_ty); (aux_tag, idx_ty tbl_ty)]).
-
-      Ltac NoDup_map_record_sort :=
-        eapply Permutation_NoDup;
-        [ eapply Permutation_map, Permuted_record_sort
-        | cbn; repeat constructor; intuition idtac;
-          destruct_In; auto ].
 
       Ltac apply_transf_to_idx_preserve_ty''_IH :=
         lazymatch goal with IH: context[type_of _ _ ?e _ ] |- type_of _ _ ?e _ => apply IH end.
@@ -220,9 +214,9 @@ Section WithMap.
           map.get Gstore tbl = Some tbl_ty ->
           is_tbl_ty tbl_ty = true ->
           type_of Gstore Genv e t ->
-          type_of (map.put Gstore tbl (transf_to_idx_ty tbl_ty)) Genv (fold_expr create_aux_read_head e) t.
+          type_of (map.put Gstore tbl (aux_ty tbl_ty)) Genv (fold_expr create_aux_read_head e) t.
       Proof.
-        unfold transf_to_idx_ty.
+        unfold aux_ty.
         induction 5 using type_of_IH; simpl; intros.
         all: try (econstructor; eauto; apply_transf_to_idx_preserve_ty''_IH; apply tenv_wf_step; eauto with fiat2_hints).
         3: repeat apply tenv_wf_step; eauto with fiat2_hints.
@@ -258,7 +252,7 @@ Section WithMap.
           is_tbl_ty tbl_ty = true ->
           well_typed Gstore Genv c ->
           incl (get_free_vars Genv) free_vars ->
-          Gstore' = map.put Gstore tbl (transf_to_idx_ty tbl_ty) ->
+          Gstore' = map.put Gstore tbl (aux_ty tbl_ty) ->
           well_typed Gstore' Genv (transf_to_idx' free_vars c).
       Proof.
         induction c; simpl; intros; try invert_well_typed; try now (constructor; auto).
@@ -302,33 +296,6 @@ Section WithMap.
         1:{ econstructor; eauto using transf_to_idx_preserve_ty''.
             use_transf_to_idx_preserve_ty'_IH; eauto with fiat2_hints.
             eauto using incl_tran, incl_cons_step, get_free_vars_put. }
-      Qed.
-
-      Lemma transf_to_idx_preserve_ty : forall tbl_ty e c free_vars Gstore Genv,
-          tenv_wf Gstore -> tenv_wf Genv ->
-          type_of Gstore Genv e tbl_ty ->
-          well_typed (map.put Gstore tbl tbl_ty) Genv c ->
-          is_tbl_ty tbl_ty = true ->
-          incl (get_free_vars Genv) free_vars ->
-          well_typed Gstore Genv (transf_to_idx free_vars (CLetMut e tbl c)).
-      Proof.
-        simpl; intros. subst. econstructor.
-        1:{ econstructor.
-            1: instantiate (1:=[(id_tag, tbl_ty); (aux_tag, idx_ty tbl_ty)]); reflexivity.
-            1:{ cbn; repeat constructor; auto.
-                eapply substitute_preserve_ty with (Genv0:=map.put map.empty hole tbl_ty); eauto using incl_refl with fiat2_hints.
-            1: eapply type_of_strengthen; [ apply to_idx_ty; eauto | apply map_incl_empty | apply map_incl_refl ].
-            1: eapply type_of__type_wf; [ | | eauto ]; auto.
-            1:{ unfold sub_wf. simpl; intros.
-                destruct_get_put_strings;
-                  [ do_injection; rewrite eqb_refl; auto
-                  | rewrite map.get_empty in *; discriminate ]. } }
-            1: eapply Permuted_record_sort.
-            1:{ cbn; repeat constructor; intuition auto. inversion H5; auto using in_nil. }
-            1: apply StronglySorted_record_sort. }
-        1:{ erewrite <- Properties.map.put_put_same.
-            eapply transf_to_idx_preserve_ty'; try reflexivity; eauto using incl_refl with fiat2_hints.
-            rewrite_map_get_put_goal; auto. }
       Qed.
 
       Definition consistent_with_global (store store' : locals) :=
@@ -600,27 +567,6 @@ Section WithMap.
             eauto using incl_tran, incl_cons_step, get_free_vars_put. }
       Qed.
 
-      Lemma transf_to_idx_preserve_sem : forall tbl_ty e c (Gstore Genv : tenv) free_vars,
-          is_tbl_ty tbl_ty = true ->
-          type_of Gstore Genv e tbl_ty ->
-          well_typed (map.put Gstore tbl tbl_ty) Genv c ->
-          incl (get_free_vars Genv) free_vars ->
-          tenv_wf Gstore -> tenv_wf Genv ->
-          forall (store env : locals),
-            locals_wf Gstore store -> locals_wf Genv env ->
-            interp_command store env (transf_to_idx free_vars (CLetMut e tbl c)) = interp_command store env (CLetMut e tbl c).
-      Proof.
-        simpl; intros.
-        apply stores_eq_except__update_eq. symmetry.
-        apply consistent_with_global__store_eq_except; auto.
-        eapply transf_to_idx_preserve_sem'; eauto with fiat2_hints.
-        1: rewrite_map_get_put_goal; auto.
-        unfold consistent_with_global; intuition idtac; repeat rewrite_map_get_put_goal.
-        erewrite NoDup_In_access_record; eauto.
-        1: NoDup_map_record_sort.
-        eapply Permutation_in; [ eapply Permuted_record_sort | ]; constructor; auto.
-      Qed.
-
       Definition aux_wf (v : value) :=
         match v with
           VRecord rv =>
@@ -665,12 +611,12 @@ Section WithMap.
             right. constructor; auto. }
       Qed.
 
-      Lemma transf_to_idx_ty_wf : forall t,
+      Lemma aux_ty_wf : forall t,
           type_wf t -> is_tbl_ty t = true ->
-          type_wf (transf_to_idx_ty t).
+          type_wf (aux_ty t).
       Proof.
         intros.
-        unfold transf_to_idx_ty. constructor; auto using StronglySorted_record_sort.
+        unfold aux_ty. constructor; auto using StronglySorted_record_sort.
         1: NoDup_map_record_sort.
         1: rewrite Forall_map.
         eapply Permutation_Forall; [ apply Permuted_record_sort | ].
@@ -719,7 +665,7 @@ Section WithMap.
           well_typed Gstore Genv c ->
         incl (get_free_vars Genv) free_vars ->
         tenv_wf Gstore -> tenv_wf Genv ->
-        parameterized_wf (map.put Gstore tbl (transf_to_idx_ty tbl_ty)) Genv (value_wf_with_globals aux_wf [tbl]) (transf_to_idx' free_vars c).
+        parameterized_wf (map.put Gstore tbl (aux_ty tbl_ty)) Genv (value_wf_with_globals aux_wf [tbl]) (transf_to_idx' free_vars c).
       Proof.
         unfold value_wf_with_globals.
         induction c; simpl; intros; try invert_well_typed; try now (constructor; auto).
@@ -746,7 +692,7 @@ Section WithMap.
                   econstructor; [ | | apply Permuted_record_sort | .. ]; auto using StronglySorted_record_sort.
                   1:{ repeat constructor; eauto using transf_to_idx_preserve_ty''.
                       eapply substitute_preserve_ty with (Genv0:=map.put map.empty hole t);
-                        eauto using transf_to_idx_ty_wf with fiat2_hints.
+                        eauto using aux_ty_wf with fiat2_hints.
                       1:{ eapply type_of_strengthen.
                           1: apply to_idx_ty; eauto with fiat2_hints.
                           1: apply map_incl_empty.
@@ -767,7 +713,7 @@ Section WithMap.
                   eapply to_idx_satisfy_idx_wf.
                   3: apply transf_to_idx_preserve_ty'';
                   [ | | eauto .. ]; auto.
-                  all: eauto using transf_to_idx_ty_wf with fiat2_hints. } }
+                  all: eauto using aux_ty_wf with fiat2_hints. } }
           1:{ econstructor.
               2: rewrite_map_get_put_goal; eauto.
               2: apply transf_to_idx_preserve_ty''; auto.
@@ -779,6 +725,164 @@ Section WithMap.
           apply_transf_to_idx'_index_wf_IH; eauto with fiat2_hints.
           eauto using incl_tran, incl_cons_step, get_free_vars_put. }
       Qed.
+      End WithGlobal.
 
+      Definition transf_to_idx (free_vars : list string) (c : command) : command :=
+        match c with
+        | CLetMut e tbl c =>
+            CLetMut (ERecord [(id_tag, e); (aux_tag, substitute ((hole, e) :: nil) free_vars to_idx)]) tbl
+              (transf_to_idx' tbl free_vars c)
+        | _ => c
+        end.
+
+      Lemma transf_to_idx_preserve_ty : forall tbl tbl_ty e c free_vars Gstore Genv,
+          tenv_wf Gstore -> tenv_wf Genv ->
+          type_of Gstore Genv e tbl_ty ->
+          well_typed (map.put Gstore tbl tbl_ty) Genv c ->
+          is_tbl_ty tbl_ty = true ->
+          incl (get_free_vars Genv) free_vars ->
+          well_typed Gstore Genv (transf_to_idx free_vars (CLetMut e tbl c)).
+      Proof.
+        simpl; intros. subst. econstructor.
+        1:{ econstructor.
+            1: instantiate (1:=[(id_tag, tbl_ty); (aux_tag, idx_ty tbl_ty)]); reflexivity.
+            1:{ cbn; repeat constructor; auto.
+                eapply substitute_preserve_ty with (Genv0:=map.put map.empty hole tbl_ty); eauto using incl_refl with fiat2_hints.
+            1: eapply type_of_strengthen; [ apply to_idx_ty; eauto | apply map_incl_empty | apply map_incl_refl ].
+            1: eapply type_of__type_wf; [ | | eauto ]; auto.
+            1:{ unfold sub_wf. simpl; intros.
+                destruct_get_put_strings;
+                  [ do_injection; rewrite eqb_refl; auto
+                  | rewrite map.get_empty in *; discriminate ]. } }
+            1: eapply Permuted_record_sort.
+            1:{ cbn; repeat constructor; intuition auto. inversion H5; auto using in_nil. }
+            1: apply StronglySorted_record_sort. }
+        1:{ erewrite <- Properties.map.put_put_same.
+            eapply transf_to_idx_preserve_ty'; try reflexivity; eauto using incl_refl with fiat2_hints.
+            rewrite_map_get_put_goal; auto. }
+      Qed.
+
+      Lemma transf_to_idx_preserve_sem : forall tbl tbl_ty e c (Gstore Genv : tenv) free_vars,
+          is_tbl_ty tbl_ty = true ->
+          type_of Gstore Genv e tbl_ty ->
+          well_typed (map.put Gstore tbl tbl_ty) Genv c ->
+          incl (get_free_vars Genv) free_vars ->
+          tenv_wf Gstore -> tenv_wf Genv ->
+          forall (store env : locals),
+            locals_wf Gstore store -> locals_wf Genv env ->
+            interp_command store env (transf_to_idx free_vars (CLetMut e tbl c)) = interp_command store env (CLetMut e tbl c).
+      Proof.
+        simpl; intros.
+        apply stores_eq_except__update_eq. symmetry.
+        eapply consistent_with_global__store_eq_except; eauto.
+        eapply transf_to_idx_preserve_sem'; eauto with fiat2_hints.
+        1: rewrite_map_get_put_goal; auto.
+        unfold consistent_with_global; intuition idtac; repeat rewrite_map_get_put_goal.
+        erewrite NoDup_In_access_record; eauto.
+        1: eapply Permutation_NoDup;
+        [ eapply Permutation_map, Permuted_record_sort
+        | cbn; repeat constructor; intuition idtac;
+          destruct_In; auto ].
+        eapply Permutation_in; [ eapply Permuted_record_sort | ]; constructor; auto.
+      Qed.
+
+      Definition apply_after_letmut f (c : command) :=
+        match c with
+        | CLetMut e x c => CLetMut e x (f x c)
+        | _ => c
+        end.
+
+      Definition apply_idx_related_transfs (f : string -> command -> command) (Gstore Genv : tenv) (c : command) :=
+        match c with
+        | CLetMut e x _ => match synthesize_expr Gstore Genv e with
+                           | Success (t, _) => if is_tbl_ty t
+                                               then apply_after_letmut f (transf_to_idx (get_free_vars Genv) c)
+                                                 else c
+                             | _ => c
+                             end
+        | _ => c
+        end.
+
+      Lemma to_idx_preserve_ty : forall Gstore Genv free_vars e t,
+          type_wf t -> is_tbl_ty t = true ->
+          tenv_wf Gstore -> tenv_wf Genv ->
+          type_of Gstore Genv e t ->
+          incl (get_free_vars Genv) free_vars ->
+          type_of Gstore Genv (substitute ((hole, e) :: nil) free_vars to_idx) (idx_ty t).
+      Proof.
+        intros. eapply substitute_preserve_ty;
+          [ | | eapply type_of_strengthen; eauto using to_idx_ty | .. ]; auto.
+        2: apply map_incl_empty.
+        2: apply map_incl_refl.
+        1: eauto with fiat2_hints.
+        1:{ unfold sub_wf; simpl; intros.
+            case_match_string_eqb; try congruence.
+            rewrite map.get_empty in *; discriminate. }
+      Qed.
+
+      Ltac apply_to_aux_preserve_ty :=
+        econstructor; [ | |  apply Permuted_record_sort | .. ];
+        auto using StronglySorted_record_sort;
+        cbn; auto; repeat constructor; intuition idtac;
+        try destruct_In; eauto;
+        apply to_idx_preserve_ty; eauto using incl_refl with fiat2_hints.
+
+      Lemma apply_idx_related_transfs_sound : forall f,
+          aug_transf_sound aux_ty aux_wf f ->
+          transf_sound (locals:=locals) (apply_idx_related_transfs f).
+      Proof.
+        unfold apply_idx_related_transfs, transf_sound; intros.
+        repeat (case_match; auto). invert_well_typed.
+        eapply synthesizable_ty_unique in E0 as H_syn_ty; eauto; subst.
+        assert (H_ty : well_typed (map.put Gstore x (aux_ty t)) Genv (transf_to_idx' x (get_free_vars Genv) c0)).
+        { erewrite <- Properties.map.put_put_same.
+          eapply transf_to_idx_preserve_ty'; try reflexivity; [ | eauto using incl_refl .. ].
+          2: rewrite_map_get_put_goal; eauto.
+          1: eauto with fiat2_hints. }
+        assert (H_wf : parameterized_wf (map.put Gstore x (aux_ty t)) Genv (value_wf_with_globals aux_wf [x]) (transf_to_idx' x (get_free_vars Genv) c0)).
+        { erewrite <- Properties.map.put_put_same.
+          apply transf_to_idx'_index_wf; eauto using incl_refl with fiat2_hints.
+          rewrite_map_get_put_goal; auto. }
+        eapply H in H_wf. 5: eauto.
+        all: eauto using aux_ty_wf with fiat2_hints.
+        2: constructor;  try eapply map.get_put_same; auto.
+        split.
+        1:{ econstructor.
+            2: apply H_wf; auto.
+            1: apply_to_aux_preserve_ty. }
+        1:{ intros. unfold transf_to_idx, apply_after_letmut.
+            cbn [interp_command]. eapply stores_eq_except__update_eq; intros.
+            destruct (map.get Gstore x0) eqn:E.
+            1:{ symmetry.
+                intuition idtac. erewrite H11; auto.
+                2:{ resolve_locals_wf. eapply type_sound.
+                    1: apply_to_aux_preserve_ty.
+                all: resolve_locals_wf; eauto using incl_refl with fiat2_hints. }
+                2:{ constructor; auto. destruct (String.eqb k x) eqn:E_kx;
+                    rewrite ?eqb_eq, ?eqb_neq in *; subst; auto; right.
+                    rewrite_map_get_put_hyp; do_injection.
+                    unfold aux_wf.
+                    repeat (erewrite NoDup_In_access_record;
+                          [
+                          | NoDup_map_record_sort
+                          | eapply Permutation_in; [ apply Permuted_record_sort | ];
+                            cbn; auto ]).
+                    eapply to_idx_satisfy_idx_wf; [ | | eauto .. ]; auto using incl_refl. }
+                eapply transf_to_idx_preserve_sem' with (Gstore:=map.put Gstore x t); eauto.
+                all: try rewrite_map_get_put_goal; eauto using incl_refl with fiat2_hints.
+                unfold consistent_with_global; intuition idtac; repeat rewrite_map_get_put_goal.
+                cbn [interp_expr].
+                erewrite NoDup_In_access_record;
+                  [
+                  | NoDup_map_record_sort
+                  | eapply Permutation_in; [ apply Permuted_record_sort | ];
+                    cbn; auto ]. reflexivity. }
+            1:{ repeat erewrite command_preserve_untouched_store. 4: eauto.
+                9: apply H_wf.
+                all: repeat rewrite_map_get_put_goal; eauto with fiat2_hints.
+                1:{ apply tenv_wf_step; eauto with fiat2_hints. apply aux_ty_wf; eauto with fiat2_hints. }
+                apply locals_wf_step; auto. eapply type_sound. 1: apply_to_aux_preserve_ty.
+                all: auto. } }
+      Qed.
     End WithIndex.
 End WithMap.
